\documentclass{zupan}

\title{Lang UG Algebra: Exercises 1}
\author{Paul Zupan}
\date{\today}

\begin{document}

\maketitle

\begin{exercise}{1}
  If $n, m$ are integers $\geq 1$ and $n \geq m$, define the \textbf{binomial
  coefficients} \[\binom{n}{m} = \frac{n!}{m!(n - m)!}.\] As usual, $n! = n
  \cdot (n - 1) \cdots 1$ is the product of the first $n$ integers. We define
  $0! = 1$ and $\binom{n}{0} = 1$. Prove that \[\binom{n}{m - 1} + \binom{n}{m}
  = \binom{n + 1}{m}.\]
\end{exercise}

\begin{solution}
  We show this using an alebraic argument:

  \[
    \begin{aligned}
      \binom{n}{m - 1} + \binom{n}{m}
        & = \frac{n!}{(m - 1)!(n - m + 1)!} + \frac{n!}{m!(n - m)!} \\
        & = \frac{n!m}{m!(n - m + 1)!} + \frac{n!(n - m + 1)}{m!(n - m + 1)!} \\
        & = \frac{n!m + n!(n - m + 1)}{m!(n - m + 1)!} \\
        & = \frac{n!(m + n - m + 1)}{m!(n - m + 1)!} \\
        & = \frac{n!(n + 1)}{m!(n + 1 - m)!} \\
        & = \frac{(n + 1)!}{m!(n + 1 - m)!} \\
        & = \binom{n + 1}{m} \\
    \end{aligned}
  \]

  Hence the identity holds as required.
\end{solution}

\begin{exercise}{2}
  Prove by induction that for any integers $x, y$ we have \[(x + y)^n = \sum_{i
  = 0}^n \binom{n}{i} x^iy^{n - i} = y^n + \binom{n}{1}xy^{n - 1} +
  \binom{n}{2}x^2y^{n - 2} + \cdots + x^n.\]
\end{exercise}

\begin{solution}
  We prove this by induction on $n$.

  TODO: Finish this problem.
\end{solution}

\end{document}
