\documentclass[12pt]{article}

\usepackage{amsmath}
\usepackage{amssymb}
\usepackage[margin=1in]{geometry}
\usepackage{parskip}

\newenvironment{exercise}{\paragraph{Exercise.}}{}
\newenvironment{solution}{\paragraph{Solution.}}{}

\newcommand{\C}{\mathbb{C}}

\begin{document}

\begin{exercise}
  Show that $\alpha + \beta = \beta + \alpha$ for all $\alpha, \beta \in \C$.
\end{exercise}

\begin{solution}
  Let $\alpha = (a_1, b_1)$ and $\beta = (a_2, b_2)$ be complex numbers.

  \[
    \begin{split}
      \alpha + \beta
        & = (a_1, b_1) + (a_2, b_2) = (a_1 + a_2, b_1 + b_2) \\
        & = (a_2 + a_1, b_2 + b_1) = (a_2, b_2) + (a_1, b_1) \\
        & = \beta + \alpha                                   \\
    \end{split}
  \]
\end{solution}

\begin{exercise}
  Show that $(\alpha + \beta) + \lambda = \alpha + (\beta + \lambda)$ for all
  $\alpha, \beta, \lambda \in \C$.
\end{exercise}

\begin{solution}
  Let $\alpha = (a_1, b_1)$, $\beta = (a_2, b_2)$, and $\lambda = (a_3, b_3)$
  be complex numbers.

  \[
    \begin{split}
      (\alpha + \beta) + \lambda
        & = ((a_1, b_1) + (a_2, b_2)) + (a_3, b_3) = (a_1 + a_2, b_1 + b_2) + (a_3, b_3)    \\
        & = ((a_1 + a_2) + a_3, (b_1 + b_2) + b_3) = (a_1 + (a_2 + a_3), b_1 + (b_2 + b_3)) \\
        & = (a_1, b_1) + (a_2 + a_3, b_2 + b_3) = (a_1, b_1) + ((a_2, b_2) + (a_3, b_3))    \\
        & = \alpha + (\beta + \lambda)                                                      \\
    \end{split}
  \]
\end{solution}

\begin{exercise}
  Show that $(\alpha\beta)\lambda = \alpha(\beta\lambda)$ for all $\alpha,
  \beta, \lambda \in \C$.
\end{exercise}

\begin{solution}
  Let $\alpha = (a_1, b_1)$, $\beta = (a_2, b_2)$, and $\lambda = (a_3, b_3)$
  be complex numbers.

  \[
    \begin{split}
      (\alpha\beta)\lambda
        & = ((a_1, b_1)(a_2, b_2))(a_3, b_3)                                                                               \\
        & = (a_1a_2 - b_1b_2, a_1b_2 + a_2b_1)(a_3, b_3)                                                                   \\
        & = ((a_1a_2 - b_1b_2)a_3 - (a_1b_2 + a_2b_1)b_3, (a_1a_2 - b_1b_2)b_3 + (a_1b_2 + a_2b_1)a_3)                     \\
        & = ((a_1a_2)a_3 - (b_1b_2)a_3 - (a_1b_2)b_3 - (a_2b_1)b_3, (a_1a_2)b_3 - (b_1b_2)b_3 + (a_1b_2)a_3 + (a_2b_1)a_3) \\
        & = (a_1(a_2a_3) - b_1(b_2a_3) - a_1(b_2b_3) - a_2(b_1b_3), a_1(a_2b_3) - b_1(b_2b_3) + a_1(b_2a_3) + a_2(b_1a_3)) \\
    \end{split}
  \]

  TODO: Finish this dumb problem
\end{solution}

\begin{exercise}
  Show that $\lambda(\alpha + \beta) = \lambda\alpha + \lambda\beta$ for all
  $\lambda, \alpha, \beta \in \C$.
\end{exercise}

\begin{solution}
  Let $\alpha = (a, b)$, $\beta = (c, d)$, and $\lambda = (e, f)$ be complex
  numbers.

  \[
    \begin{split}
      \lambda(\alpha + \beta) & = (e, f)((a, b) + (c, d))                    \\
                              & = (e, f)(a + c, b + d)                       \\
                              & = (e(a + c) - f(b + d), e(b + d) + f(a + c)) \\
                              & = (ea + ec - fb - fd, eb + ed + fa + fc)     \\
                              & = (ea - fb, eb + fa) + (ec - fd, ed + fc)    \\
                              & = (e, f)(a, b) + (e, f)(c, d)                \\
                              & = \lambda\alpha + \lambda\beta               \\
    \end{split}
  \]
\end{solution}

\begin{exercise}
  Show that for every $\alpha \in \C$, there exists a unique $\beta \in \C$
  such that $\alpha + \beta = 0$.
\end{exercise}

\begin{solution}
  Let $\alpha = (a, b)$ be a complex number. Choose $\beta = (-a, -b)$.

  \[
    \begin{split}
      \alpha + \beta & = (a, b) + (-a, -b)    \\
                     & = (a + (-a), b + (-b)) \\
                     & = (0, 0)               \\
                     & = 0                    \\
    \end{split}
  \]

  The uniqueness of $\beta$ follows from the fact that every real number has a
  unique additive inverse.
\end{solution}

\begin{exercise}
  Show that for every $\alpha \in \C$ with $\alpha \neq 0$, there exists a
  unique $\beta \in \C$ such that $\alpha\beta = 1$.
\end{exercise}

\begin{solution}
  Let $\alpha = (a, b)$ be a complex number. Choose $\beta = (\frac{a}{a^2 +
  b^2}, -\frac{b}{a^2 + b^2})$.

  \[
    \begin{split}
      \alpha\beta & = (a, b)\left(\frac{a}{a^2 + b^2}, -\frac{b}{a^2 + b^2}\right) \\
                  & = \left(\frac{a^2}{a^2 + b^2} + \frac{b^2}{a^2 + b^2},
                      -\frac{ab}{a^2 + b^2} + \frac{ab}{a^2 + b^2}\right)          \\
                  & = \left(\frac{a^2 + b^2}{a^2 + b^2}, 0\right)                  \\
                  & = (1, 0)                                                       \\
                  & = 1                                                            \\
    \end{split}
  \]
\end{solution}

\end{document}
